isabelle/core/CoreTypecheck.thy
@@ -208,13 +208,13 @@ function core_term_type :: "CoreTyEnv \<Rightarrow> GhostOrNot \<Rightarrow> Cor
         else if ghost = NotGhost \<and> (\<not> list_all (is_runtime_type env) tyArgs \<or> FI_Ghost funInfo = Ghost)
              then None
         \<comment> \<open>Term-level calls must be pure: no Ref arguments, not impure\<close>
-        else if \<not> list_all (\<lambda>(_, vor). vor = Var) (FI_TmArgs funInfo) then None
+        else if \<not> list_all (\<lambda>(_, _, vor). vor = Var) (FI_TmArgs funInfo) then None
         else if FI_Impure funInfo then None
         \<comment> \<open>Check number of term arguments\<close>
         else if length tmArgs \<noteq> length (FI_TmArgs funInfo) then None
         else
           let tySubst = fmap_of_list (zip (FI_TyArgs funInfo) tyArgs);
-              expectedArgTypes = map (\<lambda>(ty, _). apply_subst tySubst ty) (FI_TmArgs funInfo)
+              expectedArgTypes = map (\<lambda>(_, ty, _). apply_subst tySubst ty) (FI_TmArgs funInfo)
           in \<comment> \<open>Check each term argument has the expected type\<close>
              if list_all2 (\<lambda>tm expectedTy.
                    case core_term_type env ghost tm of
@@ -978,16 +978,16 @@ next
     tyargs_wk: "list_all (is_well_kinded env) tyArgs" and
     len_tmargs: "length tmArgs = length (FI_TmArgs funInfo)" and
     not_impure: "\<not> FI_Impure funInfo" and
-    all_var: "list_all (\<lambda>(_, vor). vor = Var) (FI_TmArgs funInfo)" and
+    all_var: "list_all (\<lambda>(_, _, vor). vor = Var) (FI_TmArgs funInfo)" and
     la2: "list_all2 (\<lambda>tm expectedTy.
         case core_term_type env ghost tm of None \<Rightarrow> False | Some actualTy \<Rightarrow> actualTy = expectedTy)
-        tmArgs (map (\<lambda>(ty, _). apply_subst (fmap_of_list (zip (FI_TyArgs funInfo) tyArgs)) ty)
+        tmArgs (map (\<lambda>(_, ty, _). apply_subst (fmap_of_list (zip (FI_TyArgs funInfo) tyArgs)) ty)
                     (FI_TmArgs funInfo))" and
     ty_eq: "ty = apply_subst (fmap_of_list (zip (FI_TyArgs funInfo) tyArgs)) (FI_ReturnType funInfo)"
     by (auto simp: Let_def split: option.splits if_splits)
   have la2': "list_all2 (\<lambda>tm expectedTy.
       case core_term_type ?env_x ghost tm of None \<Rightarrow> False | Some actualTy \<Rightarrow> actualTy = expectedTy)
-      tmArgs (map (\<lambda>(ty, _). apply_subst (fmap_of_list (zip (FI_TyArgs funInfo) tyArgs)) ty)
+      tmArgs (map (\<lambda>(_, ty, _). apply_subst (fmap_of_list (zip (FI_TyArgs funInfo) tyArgs)) ty)
                   (FI_TmArgs funInfo))"
     using la2 IH by (auto simp: list.rel_mono_strong split: option.splits)
   have fn_lookup': "fmlookup (TE_Functions ?env_x) fnName = Some funInfo"
